CSR_float.v
@@ -1,7 +1,7 @@
 Set Implicit Arguments.
 From SLF Require Import LabType Fun LibSepFmap Sum.
 From SLF Require Import LibWP LibSepSimpl LibSepReference LibSepTLCbuffer ListCommon.
-From SLF Require Import Struct Loops Unary_IndexWithBounds Subst NTriple Loops2 Struct2 Loops2_float Struct SV_float.
+From SLF Require Import Struct Loops Unary Subst NTriple Loops2 Struct2 Loops2_float Struct SV_float.
 From mathcomp Require Import ssreflect ssrfun zify.
 Hint Rewrite conseq_cons' : rew_listx.
 
